Add Index method for xi rope

xi-rope.dfy
@@ -1,8 +1,8 @@
 module Rope {
-  const MAX_CHILDREN: nat
-  const MIN_CHILDREN: nat
-  const MAX_LEAF_LEN: nat
-  const MIN_LEAF_LEN: nat   // minimum size requirement when splitting
+  const MAX_CHILDREN: nat := 4
+  const MIN_CHILDREN: nat := 2
+  const MAX_LEAF_LEN: nat := 10
+  const MIN_LEAF_LEN: nat := 2   // minimum size requirement when splitting
 
   datatype Node = Leaf(value: string) | InternalNode(children: seq<Rope>)
 
@@ -47,12 +47,14 @@ module Rope {
       reads this, Repr
     {
       match this.val
-      case Leaf(v) => this.len == |v|
-      case InternalNode(children) => this.len == this.Len()
+      case Leaf(v) => this.len == |v| && ContentLen(this.Content) == |v| && |Content| == 1
+      case InternalNode(children) => this.len == this.Len() && forall c: Rope :: c in children ==> c.len <= this.len && c.ValidLen()
     }
 
     predicate Valid()
       reads this, Repr
+      requires MAX_LEAF_LEN >= MIN_LEAF_LEN
+      requires MIN_CHILDREN <= MAX_CHILDREN && MIN_CHILDREN >= 2
     {
       this in Repr &&
       (
@@ -62,369 +64,52 @@ module Rope {
           (HasParent ==>
             |children| >= MIN_CHILDREN &&
             |children| <= MAX_CHILDREN &&
-            forall c: Rope :: c in children ==> c in Repr && this !in c.Repr && c.Repr <= Repr && c.Valid() && c.Content <= Content
+            forall c: Rope :: c in children ==> c in Repr && this !in c.Repr && c.Repr <= Repr && c.Valid() && c.Content <= Content && forall cont: string :: cont in c.Content ==> cont in this.Content
           ) &&
           (!HasParent ==>
             |children| >= 2 &&
             |children| <= MAX_CHILDREN &&
-            forall c: Rope :: c in children ==> c in Repr && this !in c.Repr && c.Repr <= Repr && c.Valid() && c.Content <= Content
+            forall c: Rope :: c in children ==> c in Repr && this !in c.Repr && c.Repr <= Repr && c.Valid() && c.Content <= Content && forall cont: string :: cont in c.Content ==> cont in this.Content
           )
       )
     }
-  }
-}
 
-
-----
-
-
-const max: int
-const min: int
-
-datatype Node<T> = Leaf(value: T) | InternalNode(children: seq<Rope<T>>)
-
-class Rope<T> {
-  ghost var Repr: set<object>
-
-  var val: Node<T>
-  var len: int
-
-  predicate Valid()
-    reads this, Repr
-  {
-    this in Repr &&
-    (
-      match this.val
-      case Leaf(v) => true
-      case InternalNode(children) =>
-        |children| >= min &&
-        |children| <= max &&
-        (forall i :: 0 <= i < |children| ==> children[i] in Repr && Repr >= children[i].Repr && this !in children[i].Repr && children[i].Valid())
-    )
-  }
-
-  constructor Init(v: T)
-  {
-    val := Leaf(v);
-    len := 0;
-    Repr := {this};
-  }
-}
-
-----
-
-
-module Rope {
-  datatype Node<T> = Leaf(value: T) | InternalNode(children: seq<Rope<T>>)
-
-  class Rope<T> {
-    var val: Node<T>
-    var len: int
-    var max: int
-    var min: int
-
-
-    function sum<T>(c: seq<Rope<T>>): int
-      requires |c| > 0
+    method Index(i: int) returns (charAtIndex: string)
+      requires Valid()
+      requires ValidLen()
+      //ensures i >= 0 && i < this.len ==> charAtIndex != ""
+      ensures i < 0 || i >= this.len ==> charAtIndex == ""
+      decreases Repr
     {
-      if |c| == 1 then countLeaves(c[0])
-      else countLeaves(c[0]) + sum(c[1..])
+      if this.len <= i || i < 0
+        { charAtIndex := ""; }
+      else
+        {
+          match this.val
+          case Leaf(v) =>
+            charAtIndex := [v[i]];
+          case InternalNode(children) =>
+            var c := 0;
+            var newI := i;
+
+            while (c + 1 < |children| && children[c].len <= newI)
+              invariant 0 <= c < |children|
+              {
+                newI := newI - children[c].len;
+                c := c + 1;
+              }
+
+            charAtIndex := children[c].Index(newI);
+        }
     }
 
-
-    function countLeaves(r: Rope): int
-      decreases r
-    {
-      match r
-      case Leaf(v) => 1
-      case Node(children) =>
-        if |children| <= 0 then 0
-        else sum(children)
-    }
+//    function method SliceToString(i: int, j: int): string
+//      requires Valid()
+//      requires ValidLen()
+//      reads this
+//      // todo ensures
+//    {
+//        // todo
+//    }
   }
-}
-
-
-class Node {
-  ghost var Contents: set<int>
-  ghost var Repr: set<object>
-
-  var data: int
-  var nodes: set<Node>
-
-  predicate Valid()
-    reads this, Repr
-  {
-    this in Repr &&
-    (|nodes| > 0 ==>
-      forall n :: n in nodes ==> n in Repr && n.Repr <= Repr && this !in n.Repr && n.Valid()
-    ) &&
-    (|nodes| == 0 ==>
-      Contents == {data})
-  }
-}
-
-
-module Rope {
-  datatype Node<T> = Leaf(value: T) | InternalNode(children: seq<Rope<T>>)
-
-  class Rope<T> {
-    var val: Node<T>
-    var len: int
-    var max: int
-    var min: int
-
-
-    function sum<T>(c: seq<Rope<T>>): int
-      reads c
-      requires |c| > 0
-      decreases c
-    {
-      if |c| == 1 then c[0].countLeaves()
-      else c[0].countLeaves() + sum(c[1..])
-    }
-
-
-    function countLeaves(): int
-      reads this
-      decreases this.val
-    {
-      match this.val
-      case Leaf(v) => 1
-      case InternalNode(children) =>
-        if |children| <= 0 then 0
-        else this.sum(children)
-    }
-  }
-}
-
-
-
-
-
-predicate validChildren(rope: Rope<T>)
-  reads rope
-{
-  match rope.val
-  case Leaf(t) => true    // todo: all children must be either leaves or internal nodes? not mixed?
-  case InternalNode(children) => |children| >= min && |children| <= max && forall k: int :: 0 <= k < |children| ==> validChildren(children[k])
-}
-
-
-
-
-predicate childCount(rope: Rope<T>)
-  reads rope
-{
-  match rope.val
-  case Leaf(t) => true
-  case InternalNode(children) => forall k: int :: 0 <= k < children.Length ==> minChildren(a[k])
-}
-
-
-
-
-datatype Rope<T> = Leaf(value: T) | Node(children: seq<Rope<T>>)
-
-function sum<T>(c: seq<Rope<T>>): int
-  requires |c| > 0
-{
-  if |c| == 1 then countLeaves(c[0])
-  else countLeaves(c[0]) + sum(c[1..])
-}
-
-
-function countLeaves(r: Rope): int
-  decreases r
-{
-  match r
-  case Leaf(v) => 1
-  case Node(children) =>
-    if |children| <= 0 then 0
-    else sum(children)
-}
-
-
-
-module Rope {
-  datatype Node<T> = Leaf(value: T) | InternalNode(children: seq<Rope<T>>)
-
-  class Rope<T> {
-    var val: Node<T>
-    var len: int
-    var max: int
-    var min: int
-
-    function sum<T>(c: seq<Rope<T>>): int
-      reads c
-      decreases |c|
-    {
-      if |c| == 0 then 0
-      else if |c| == 1 then c[0].countLeaves()
-      else c[0].countLeaves() + sum(c[1..])
-    }
-
-
-    function countLeaves(): int
-      reads this
-      decreases this
-    {
-      match this.val
-      case Leaf(v) => 1
-      case InternalNode(children) => sum(children)
-    }
-  }
-}
-
-
-module Rope {
-  datatype Node<T> = Leaf(value: T) | InternalNode(children: seq<Rope<T>>)
-
-  class Rope<T> {
-    var val: Node<T>
-    var len: int
-    var max: int
-    var min: int
-
-    predicate childCount(rope: Rope<T>)
-      reads rope
-    {
-      match rope.val
-      case Leaf(t) => true
-      case InternalNode(children) => forall k: int :: 0 <= k < |rope.val.children| ==> minChildren(rope.val.children[k])
-    }
-
-    predicate minChildren(rope: Rope<T>)
-      reads rope
-    {
-      match rope.val
-      case Leaf(t) => true
-      case InternalNode(children) => |rope.val.children| >= min && forall k: int :: 0 <= k < |rope.val.children| ==> minChildren(rope.val.children[k])
-    }
-
-  }
-}
-
-
-
-
-
-datatype Rope<T> = Leaf(value: T) | Node(children: seq<Rope<T>>)
-
-function sum<T>(q: seq<Rope<T>>): int
-  requires |q| > 0
-{
-  if |q| == 1 then toList(1, q[0])
-  else toList(1, q[0]) + sum(q[1..])
-}
-
-
-function toList(d: int, t: Rope): int
-  decreases t
-{
-  match t
-  case Leaf(v) => d
-  case Node(children) =>
-    if |children| <= 0 then d
-    else sum(children)
-}
-
-
-
-
-
-
-
-
-predicate childCount(rope: Rope<T>)
-  reads rope
-{
-  match rope
-  case Leaf(t) => true
-  case
-}
-
-
-
-const max: int
-const min: int
-
-datatype Node<T> = Leaf(value: T) | InternalNode(children: seq<Rope<T>>)
-
-class Rope<T> {
-  ghost var Repr: set<object>
-
-  var val: Node<T>
-  var len: int
-
-  predicate Valid()
-    reads this, Repr
-  {
-    this in Repr &&
-    (
-      match this.val
-      case Leaf(v) => true
-      case InternalNode(children) =>
-        |children| >= min &&
-        |children| <= max &&
-        (forall i :: 0 <= i < |children| ==> children[i] in Repr && this !in children[i].Repr && children[i].Valid())
-    )
-  }
-
-  constructor Init(v: T)
-  {
-    val := Leaf(v);
-    len := 0;
-    Repr := {this};
-  }
-
-}
-
-
-
-
-
-lemma countLemma(rope: Rope<T>, i: int)
-   requires i >= 0 && i < 5
-   ensures rope.Node? && (LeafCount(Node(rope.children[0..i-1], i - 1) + LeafCount(rope.children[i], 1) == LeafCount(rope, i)
-{
-
-}
-
-datatype Rope<T> = Leaf(value: T) | Node(children: seq<Rope<T>>)
-
-function rec(t: Rope): seq<int> {
-  match t
-  case Leaf(v) => 1
-  case Node(children) =>
-    if |children| <= 0 then 1
-    else toList(d+1, children[0]) + toList(d+1, Node(children[1..]))
-}
-
-function toList(d: int, t: Rope): seq<int>
-  decreases t
-{
-  match t
-  case Leaf(v) => [d]
-  case Node(children) =>
-    if |children| == 0 then [d]
-    else toList(d+1, children[0]) + toList(d+1, Node(children[1..]))
-}
-
-
-function LeafCount<T>(rope: Rope<T>, i: int): int {
-    match rope
-    case Leaf(t) => 1
-    case Node(children) =>
-      if |children| == 0 || i == 0 then 0
-      else LeafCount(children[0], 5) + LeafCount(Node(children[1..]), i - 1)
-}
-
-
-
-lemma sumLemma(s: seq<int>, i: int)
-   requires i >= 0 && i < |s|
-   ensures (sum(s, i) + s[i]) == sum(s, i + 1)
-{
-
 }
